gitignore

pset2/Pset2.v
@@ -1,9 +1,663 @@
-(** * 6.887 Formal Reasoning About Programs, Spring 2016 - Pset 2 *)
+`(** * 6.887 Formal Reasoning About Programs, Spring 2016 - Pset 2 *)
 
 Require Import Frap Pset2Sig.
+
+Definition contribution_from (pr : increment_program) : nat :=
+  match pr with
+  | UnsetFlag => 1
+  | Done => 1
+  | _ => 0
+  end.
+
+Definition flag_set (pr : increment_program) : bool :=
+  match pr with
+  | SetFlag => false
+  | SetTurn => true
+  | ReadFlag => true
+  | ReadTurn => true
+  | Read => true
+  | Write _ => true
+  | UnsetFlag => true
+  | Done => false 
+  end.
+
+
+Definition is_valid_turn (pr1 pr2: increment_program) (turn: bool) :=
+   match pr1 with
+     | SetFlag => match pr2 with
+                    | _ => match turn with
+                          | true => False
+                          | false => True
+                           end
+                    end
+     | SetTurn => match pr2 with
+                    | _ => match turn with
+                          | true => False
+                          | false => True
+                           end
+                  end
+     | ReadFlag => match pr2 with
+                    |SetFlag => match turn with
+                                  |true => True
+                                  |false => False
+                                 end
+                    |SetTurn => match turn with
+                                 |true => True
+                                  |false => False
+                                 end
+                    |ReadFlag => match turn with
+                                  |_ => True
+                                 end
+                    |ReadTurn => match turn with
+                                  |_ => True
+                                 end
+                    |Read => match turn with
+                                  |true => True
+                                  |false => False
+                                 end
+                    |Write n => match turn with
+                                  |true => True
+                                  |false => False
+                                 end
+                    |UnsetFlag => match turn with
+                                  |true => True
+                                  |false => False
+                                 end
+                    |Done => match turn with
+                                  |true => True
+                                  |false => False
+                                 end
+                    end
+  | ReadTurn => match pr2 with
+                    |SetFlag => match turn with
+                                  |true => True
+                                  |false => False
+                                 end
+                    |SetTurn => match turn with
+                                 |true => True
+                                  |false => False
+                                 end
+                    |ReadFlag => match turn with
+                                  |_ => True
+                                 end
+                    |ReadTurn => match turn with
+                                  |_ => True
+                                 end
+                    |Read => match turn with
+                                  |true => True
+                                  |false => False
+                                 end
+                    |Write n => match turn with
+                                  |true => True
+                                  |false => False
+                                 end
+                    |UnsetFlag => match turn with
+                                  |true => True
+                                  |false => False
+                                 end
+                    |Done => match turn with
+                                  |true => True
+                                  |false => False
+                                 end
+                    end
+  | Read => match pr2 with
+                    |SetFlag => match turn with
+                                  |true => True
+                                  |false => False
+                                 end
+                    |SetTurn => match turn with
+                                  |true => True
+                                  |false => False
+                                 end
+                    |ReadFlag => match turn with
+                                  |true => False
+                                  |false => True
+                                 end
+                    |ReadTurn => match turn with
+                                  |true => False
+                                  |false => True
+                                 end
+                    |Read => False
+                    |Write n => False
+                    |UnsetFlag => False
+                    |Done => match turn with
+                                  |true => True
+                                  |false => False
+                                 end
+                    end
+  | Write _ => match pr2 with
+                    |SetFlag => match turn with
+                                  |true => True
+                                  |false => False
+                                 end
+                    |SetTurn => match turn with
+                                  |true => True
+                                  |false => False
+                                 end
+                    |ReadFlag => match turn with
+                                  |true => False
+                                  |false => True
+                                 end
+                    |ReadTurn => match turn with
+                                  |true => False
+                                  |false => True
+                                 end
+                    |Read => False
+                    |Write n => False
+                    |UnsetFlag => False
+                    |Done => match turn with
+                                  |true => True
+                                  |false => False
+                                 end
+                    end
+  | UnsetFlag => match pr2 with
+                    |SetFlag => match turn with
+                                  |true => True
+                                  |false => False
+                                 end
+                    |SetTurn => match turn with
+                                  |true => True
+                                  |false => False
+                                 end
+                    |ReadFlag => match turn with
+                                  |true => False
+                                  |false => True
+                                 end
+                    |ReadTurn => match turn with
+                                  |true => False
+                                  |false => True
+                                 end
+                    |Read => False
+                    |Write n => False
+                    |UnsetFlag => False
+                    |Done => match turn with
+                                  |true => True
+                                  |false => False
+                                 end
+                    end
+  | Done => match pr2 with
+                    |SetFlag => match turn with
+                                  |true => True
+                                  |false => False
+                                 end
+                    |SetTurn => match turn with
+                                  |true => True
+                                  |false => False
+                                 end
+                    |ReadFlag => match turn with
+                                  |true => False
+                                  |false => True
+                                 end
+                    |ReadTurn => match turn with
+                                 |true => False
+                                  |false => True
+                                 end
+                    |Read => match turn with
+                                  |true => False
+                                  |false => True
+                                 end
+                    |Write n => match turn with
+                                  |true => False
+                                  |false => True
+                                 end
+                    |UnsetFlag => match turn with
+                                  |true => False
+                                  |false => True
+                                 end
+                    |Done => True
+                    end
+   end.
+
+Definition in_cs (pr : increment_program) : bool :=
+  match pr with
+  | SetFlag => false
+  | SetTurn => false 
+  | ReadFlag => false
+  | ReadTurn => false
+  | Read => true
+  | Write n => true
+  | UnsetFlag => true
+  | Done => false
+  end.           
+Definition shared_from_private (pr1 pr2 : increment_program) (turn : bool):=
+  {| Flag1 := flag_set pr1;
+     Flag2 := flag_set pr2;
+     Turn := turn;
+     Global := contribution_from pr1 + contribution_from pr2 |}.
+
+(*both not in CS*)
+Definition instruction_ok (self other : increment_program) :=
+  match self with
+  | SetFlag => True
+  | SetTurn => True
+  | ReadFlag => True
+  | ReadTurn => True
+  | Read => in_cs other = false 
+  | Write n => in_cs other = false /\ n = contribution_from other
+  | UnsetFlag => in_cs other = false 
+  | Done => True
+  end.
+
+Inductive increment2_invariant :
+  threaded_state inc_state (increment_program * increment_program) -> Prop :=
+| Inc2Inv : forall pr1 pr2 turn,
+  instruction_ok pr1 pr2
+  -> instruction_ok pr2 pr1
+  -> is_valid_turn pr1 pr2 turn
+  -> increment2_invariant {| Shared := {|Flag1 := flag_set pr1;
+                                         Flag2 := flag_set pr2;
+                                         Turn := turn;
+                                         Global := contribution_from pr1 + contribution_from pr2|}; Private := (pr1, pr2) |}.
+
+
+Definition shared_from_private1 (pr1 pr2 : increment_program) (turn : bool) :=
+  {|Flag1 := flag_set pr1;
+    Flag2 := flag_set pr2;
+    Turn := turn;
+    Global := contribution_from pr1 + contribution_from pr2 |}.
+
+Lemma Inc2Inv' : forall sh pr1 pr2 turn,
+   sh = shared_from_private1 pr1 pr2 turn 
+   -> instruction_ok pr1 pr2
+   -> instruction_ok pr2 pr1
+   -> is_valid_turn pr1 pr2 turn
+   -> increment2_invariant {| Shared := sh; Private := (pr1, pr2) |}.
+Proof.
+  intros.
+  rewrite H.
+  apply Inc2Inv; assumption.
+Qed.
+
+Theorem increment2_invariant_ok : invariantFor increment2_sys increment2_invariant.
+Proof.
+  apply invariant_induction; simplify.
+  invert H.
+  invert H0.
+  invert H1.
+
+  eapply Inc2Inv'.
+
+  unfold shared_from_private1.
+  simplify.
+  equality.
+
+  simplify.
+  propositional.
+
+  simplify.
+  propositional.
+
+  simplify.
+  propositional.
+
+  invert H.
+  invert H0.
+  invert H7; simplify.
+
+  cases pr2; simplify.
+  
+  eapply Inc2Inv'; unfold shared_from_private1; simplify.
+  equality.
+  equality.
+  equality.
+
+  apply H3.
+
+  eapply Inc2Inv'; unfold shared_from_private1; simplify.
+  equality.
+  equality.
+  equality.
+  equality.
+
+  eapply Inc2Inv'; unfold shared_from_private1; simplify.
+  equality.
+  equality.
+  equality.
+  equality.
+
+  eapply Inc2Inv'; unfold shared_from_private1; simplify.
+  equality.
+  equality.
+  equality.
+  equality.
+
+  eapply Inc2Inv'; unfold shared_from_private1; simplify.
+  equality.
+  equality.
+  equality.
+  equality.
+
+  eapply Inc2Inv'; unfold shared_from_private1; simplify.
+  equality.
+  equality.
+  equality.
+  equality.
+
+
+  eapply Inc2Inv'; unfold shared_from_private1; simplify.
+  equality.
+  equality.
+  equality.
+  equality.
+
+
+  eapply Inc2Inv'; unfold shared_from_private1; simplify.
+  equality.
+  equality.
+  equality.
+  equality.
+
+  eapply Inc2Inv'; unfold shared_from_private1; simplify.
+  equality.
+  equality.
+  equality.
+  
+  cases pr2; equality.
+
+  eapply Inc2Inv'; unfold shared_from_private1; simplify.
+  equality.
+  equality.
+  equality.
+
+  apply H3.
+  simplify.
+  eapply Inc2Inv'; unfold shared_from_private1; simplify.
+  equality.
+  unfold in_cs.
+  cases pr2; equality.
+
+  unfold instruction_ok.
+  cases pr2; trivial.
+
+  unfold in_cs.
+  simplify.
+  equality.
+
+  cases pr2.
+  apply H3.
+  apply H3.
+  simplify.
+  equality.
+
+  simplify.
+  simplify.
+  equality.
+
+  simplify.
+  equality.
+
+  simplify.
+  equality.
+  
+  simplify.
+  equality.
+  apply H3.
+
+  eapply Inc2Inv'; unfold shared_from_private1; simplify.
+  equality.
+  equality.
+  equality.
+
+  cases pr2; trivial.
+  
+  eapply Inc2Inv'; unfold shared_from_private1; simplify.
+  equality.
+  unfold in_cs.
+  cases pr2; trivial.
+  equality.
+  equality.
+  simplify.
+  equality.
+
+  unfold instruction_ok.
+  cases pr2; trivial.
+
+  unfold in_cs.
+  equality.
+
+  unfold in_cs.
+  unfold contribution_from.
+  equality.
+
+  unfold in_cs.
+  equality.
+
+  cases pr2; trivial.
+
+  eapply Inc2Inv'; unfold shared_from_private1; simplify.
+  equality.
+  equality.
+  equality.
+
+  cases pr2; trivial.
+
+  eapply Inc2Inv'; unfold shared_from_private1; simplify.
+  unfold contribution_from.
+  cases pr2.
+  simplify.
+
+  invert H1.
+  equality.
+
+  invert H1.
+  unfold contribution_from.
+  equality.
+
+  invert H1.
+  unfold contribution_from.
+  equality.
+
+  invert H1.
+  unfold contribution_from.
+  equality.
+
+  invert H1.
+  unfold contribution_from.
+  equality.
+  
+  equality.
+  equality.
+
+  invert H1.
+  unfold contribution_from.
+  equality.
+
+  eapply H1.
+  unfold instruction_ok.
+  cases pr2; trivial.
+  invert H1.
+  invert H.
+  apply H3.
+
+  eapply Inc2Inv'; unfold shared_from_private1; simplify.
+  unfold contribution_from.
+  equality.
+  equality.
+
+  unfold instruction_ok.
+  cases pr2; trivial.
+  invert H1.
+  cases pr2; repeat apply H3.
+  equality.
+  equality.
+  equality.
+  equality.
+ 
+  (* *)
+  (**** THIS is where I was stuck, I originally had eapply, and then invert, 
+   but that lead to the weir turn = true, turn = false cases
+   switching the order helped me avoid that.****)
+  invert H7.
+  eapply Inc2Inv'; unfold shared_from_private1; simplify.
+ 
+  simplify.
+  equality.
+
+  unfold instruction_ok.
+  simplify.
+  cases pr1.
+  equality.
+  equality.
+  equality.
+  equality.
+  equality.
+  trivial.
+  equality.
+  equality.
+  equality.
+  
+  unfold is_valid_turn.
+  
+  cases pr1.
+  simplify.
+  simplify.
+  apply H3.
+  simplify.
+  apply H3.
+  simplify.
+  apply H3.
+  simplify.
+  apply H3.
+  simplify.
+  apply H3.
+  simplify.
+  apply H3.
+  simplify.
+  apply H3.
+  simplify.
+  apply H3.
+
+  eapply Inc2Inv'; unfold shared_from_private1; simplify.
+
+  simplify.
+  equality.
+
+  unfold instruction_ok.
+
+  cases pr1; simplify; equality.
+  equality.
+  unfold is_valid_turn.
+  cases pr1; equality.
+
+  eapply Inc2Inv'; unfold shared_from_private1; simplify.
+
+  simplify.
+  equality.
+
+  unfold instruction_ok.
+  cases pr1; simplify; equality.
+  equality.
+
+  unfold is_valid_turn.
+  cases pr1; simplify; equality.
+
+  eapply Inc2Inv'; unfold shared_from_private1; simplify.
+
+  simplify.
+  equality.
+
+  unfold instruction_ok.
+  cases pr1; simplify; equality.
+
+  unfold in_cs.
+  cases pr1; simplify; equality.
+
+  unfold is_valid_turn.
+  cases pr1; simplify; equality.
+
+  eapply Inc2Inv'; unfold shared_from_private1; simplify.
+  simplify.
+  equality.
+
+  unfold instruction_ok.
+  cases pr1; simplify; equality.
+
+  equality.
+
+  unfold is_valid_turn.
+  cases pr1; simplify; equality.
+
+  eapply Inc2Inv'; unfold shared_from_private1; simplify.
+  equality.
+
+  unfold instruction_ok.
+  cases pr1; simplify; equality.
+
+  unfold in_cs.
+  cases pr1; simplify; equality.
+
+  unfold is_valid_turn.
+  cases pr1; simplify; equality.
+
+  eapply Inc2Inv'; unfold shared_from_private1; simplify.
+  equality.
+
+  unfold instruction_ok.
+  cases pr1;simplify; equality.
+
+  unfold contribution_from.
+
+  cases pr1; simplify; equality.
+
+  unfold is_valid_turn.
+  cases pr1; simplify; equality.
+
+  eapply Inc2Inv'; unfold shared_from_private1; simplify.
+  unfold contribution_from.
+  cases pr1; simplify.
+  invert H2.
+  equality.
+  invert H2.
+  equality.
+  invert H2.
+  equality.
+  invert H2.
+  equality.
+  invert H2.
+  equality.
+  invert H2.
+  equality.
+  invert H2.
+  equality.
+  invert H2.
+  equality.
+
+  unfold instruction_ok.
+  cases pr1; simplify; equality.
+
+  unfold in_cs.
+  cases pr1; simplify; equality.
+
+  unfold is_valid_turn.
+  cases pr1; simplify; equality.
+
+  eapply Inc2Inv'; unfold shared_from_private1; simplify.
+  equality.
+  unfold instruction_ok.
+  cases pr1; simplify; equality.
+
+  equality.
+
+  unfold is_valid_turn.
+  cases pr1; simplify; equality.
+
+Qed.
+  
+  
 
 
 Theorem increment2_ok :
   invariantFor increment2_sys increment2_correct.
 Proof.
-Admitted.
+ 
+  apply invariant_weaken with (invariant1 := increment2_invariant).
+  apply increment2_invariant_ok.
+  simplify.
+
+  invert H.
+  unfold increment2_correct; simplify.
+  invert H.
+  simplify.
+  equality.
+Qed.
+(*fcn that takes in pr1 pr2 turn and return prop *)
