pset1/Pset1.v
@@ -1,31 +1,284 @@
 (** * 6.887 Formal Reasoning About Programs, Spring 2016 - Pset 1 *)
 
-Require Import Frap Pset1Sig.
+Require Import Frap Pset1Sig.                             
 
-
+Lemma applyIndHyp : forall (x : nat) (m1: map_) (m2 : map_), (allPositive m1 -> x > 0 -> interp_map m1 x > 0) -> ( allPositive m2 -> x > 0 -> interp_map m2 x > 0) -> ( allPositive (Add m1 m2) -> x > 0 -> interp_map (Add m1 m2) x > 0).
+  Proof.
+    intros.
+    simplify.
+    destruct H1.
+    specialize (H H1 H2).
+    specialize (H0 H3 H2).
+    linear_arithmetic.
+  Qed.
 Theorem allPositive_ok : forall (m : map_) (x : nat),
   allPositive m
   -> x > 0
   -> interp_map m x > 0.
 Proof.
-Admitted.
+  
+  (*works below*)
+  induct m. intro.
+  intro.
+  intro.
+  unfold interp_map.
+  unfold allPositive in H. trivial.
 
-Theorem reduce_swap : forall e ls1 ls2, interp_reduce e (ls1 ++ ls2) = interp_reduce e (ls2 ++ ls1).
+  intro.
+  intro.
+  intro.
+  unfold allPositive in H.
+  unfold interp_map. trivial.
+
+  intro.
+  Check applyIndHyp.
+  apply (applyIndHyp x m1 m2 (IHm1 x) (IHm2 x)).
+
+  intros.
+  simplify.
+  specialize (IHm2 x).
+  specialize (IHm1 (interp_map m2 x)).
+  destruct H.
+  exact (IHm1 H (IHm2 H1 H0)).
+Qed.
+(*from perry*)
+(*
+Lemma fl_lsls_plus_ls: forall (lsls : list(list nat)) (ls1 ls2 : nat), fold_left plus lsls (ls1 ++ ls2) = fold_left plus lsls ls1 ++ ls2.
 Proof.
-Admitted.
+
+Admitted.*)
+
+Lemma fl_list_plus_nat: forall (ls : list nat) (a0 a : nat), fold_left plus ls (a0 + a) = fold_left plus ls a0 + a.
+Proof.
+  induct ls.
+  simplify.
+  ring.
+  simplify.
+  repeat rewrite IHls.
+  SearchAbout fold_left.
+  ring.
+Qed.
+
+Lemma fl_list_max_nat: forall (ls : list nat) (a0 a : nat), fold_left max ls (max a0 a) = max (fold_left max ls a0) a.
+Proof.
+  induct ls.
+  simplify.
+  ring.
+
+  simplify.
+  repeat rewrite IHls.
+  SearchAbout max.
+  
+  rewrite <- Max.max_assoc .
+  symmetry.
+  rewrite <- Max.max_assoc.
+  f_equal.
+  apply Max.max_comm.
+Qed.
+
+Lemma fl_swap_plus : forall (ls1 ls2 : list nat) (a:nat), fold_left plus (ls1 ++ ls2) a = fold_left plus (ls2 ++ ls1) a.
+Proof.
+  induct ls1.
+  simplify.
+  rewrite app_nil_r.
+  equality.
+  
+  simplify.
+  SearchAbout fold_left app.
+  rewrite IHls1.
+  repeat rewrite fold_left_app.
+  simplify.
+  f_equal.
+  apply fl_list_plus_nat.
+Qed.
+
+Lemma fl_swap_max :  forall (ls1 ls2 : list nat) (a:nat), fold_left max (ls1 ++ ls2) a = fold_left max (ls2 ++ ls1) a.
+Proof.
+  induct ls1.
+  simplify.
+  rewrite app_nil_r.
+  equality.
+
+  simplify.
+  rewrite IHls1.
+  repeat rewrite fold_left_app.
+  repeat simplify.
+  f_equal.
+  apply fl_list_max_nat.
+Qed.
+    
+Theorem reduce_swap : forall e ls1 ls2, interp_reduce e (ls1 ++ ls2) = interp_reduce e (ls2 ++ ls1).
+Proof.  
+  (*try cases, destruct, cases on +, max*)
+  induct e.
+  simplify.
+  apply fl_swap_plus.
+  repeat simplify.
+  apply fl_swap_max.
+Qed.
+
 
 Theorem interp_swap : forall e ls1 ls2, interp_mr e (ls1 ++ ls2) = interp_mr e (ls2 ++ ls1).
 Proof.
-Admitted.
+  induct e.
+  simplify.
+  unfold interp_mr.
+  simplify.
+  SearchAbout map.
+  rewrite -> map_app.
+  symmetry.
+  rewrite -> map_app.
+  simplify.
+  rewrite reduce_swap.
+  equality.  
+Qed.
 
+Lemma red_add_dist : forall(ls1 ls2 : list nat), fold_left plus (ls1 ++ ls2) 0 = fold_left plus ls1 0 + fold_left plus ls2 0. 
+Proof.
+  induct ls1.
+  induct ls2.
+  simplify.
+  equality.
+
+  simplify.
+  equality.
+
+  simplify.
+  SearchRewrite (_ + 0).
+  rewrite <- (plus_0_r (a)).
+  rewrite <- plus_comm.
+  SearchRewrite (_ + _). 
+  rewrite fl_list_plus_nat.
+  symmetry.
+  rewrite fl_list_plus_nat.
+  symmetry.
+  specialize (IHls1 ls2).
+  
+  rewrite IHls1.
+  linear_arithmetic.  
+Qed.
+
+Lemma red_max_dist : forall (ls1 ls2 : list nat), fold_left max (ls1 ++ ls2) 0 = max (fold_left max ls1 0) (fold_left max ls2 0).
+Proof.
+  induct ls1.
+  induct ls2.
+  simplify.
+  equality.
+
+  simplify.
+  equality.
+
+  simplify.
+  SearchAbout max.
+  
+  rewrite fl_list_max_nat.
+  symmetry.
+  rewrite fl_list_max_nat.
+  symmetry.
+
+  specialize (IHls1 ls2).
+  rewrite IHls1.
+  SearchAbout max.
+
+  
+  rewrite <- Max.max_assoc.
+  symmetry.
+  rewrite <- Max.max_assoc.
+  symmetry.
+  f_equal.
+  rewrite <- Max.max_comm .
+  equality.
+Qed.
 Theorem mapReduce_partition_two : forall m r ls1 ls2, interp_mr (m, r) (ls1 ++ ls2) = interp_reduce r [interp_mr (m, r) ls1; interp_mr (m, r) ls2].
 Proof.
-Admitted.
+  induct r.
+  simplify.
+  unfold interp_mr.
+  simplify.
+
+  
+  SearchAbout map.
+  rewrite map_app.
+  rewrite red_add_dist.
+  linear_arithmetic.
+
+  unfold interp_mr.
+  simplify.
+
+  rewrite map_app.
+  rewrite Max.max_0_l.
+  rewrite red_max_dist.
+  equality.
+Qed.
 
 Arguments app {_} _ _ .
+Lemma app_conc : forall a (ls : list a) (b : a), b::ls = [b]++ls.
+Proof.
+  simplify.
+  equality.
+Qed.
+
+Lemma lsls_partition : forall (lsls : list(list nat)) (a : list nat), fold_left app lsls a = fold_left app lsls [] ++ a.
+Proof.
+  
+(*
+  induct lsls.
+  simplify.
+  equality.
+
+  simplify.
+  SearchAbout app.
+  cases a.
+  simplify.
+  rewrite IHlsls.
+  SearchRewrite (_ ++ []).  
+  rewrite app_nil_r.
+  equality.
+
+  *)
+Admitted.
+
 
 Theorem mapReduce_partition : forall m r lsls, interp_mr (m, r) (fold_left app lsls []) = interp_reduce r (List.map (interp_mr (m, r)) lsls).
 Proof.
-Admitted.
+  induct lsls.
+  simplify.
+  unfold interp_mr.
+  simplify.
+  equality.
+  
+  simplify.
+
+  rewrite lsls_partition.
+  rewrite mapReduce_partition_two.
+  rewrite IHlsls.
+  rewrite app_conc.
+  rewrite reduce_swap.
+
+  cases r.
+  simplify.
+  rewrite <- (plus_0_r (interp_mr (m, Sum) a)).
+  rewrite <- plus_comm.
+  SearchRewrite (_ + _). 
+  rewrite fl_list_plus_nat.
+
+  symmetry.
+  rewrite <- (plus_0_r (interp_mr (m, Sum) a)).
+  rewrite <- (plus_comm (0) ( interp_mr (m, Sum) a)).
+  SearchRewrite (_ + 0). 
+  rewrite fl_list_plus_nat.
+  simplify.
+  linear_arithmetic.
+
+  simplify.
+  (*rewrite fl_list_max_nat.*)
+  symmetry.
+  rewrite fl_list_max_nat.
+  simplify.
+  rewrite Max.max_0_l.
+  rewrite Max.max_comm.
+  equality.
+  
+Qed.
 
 (* For full credit, the code you turn in can't use [Admitted] or [admit] anymore! *)
