pset1/Pset1Sol.v
@@ -1,0 +1,244 @@
+(** * 6.887 Formal Reasoning About Programs, Spring 2016 - Pset 1 *)
+
+Require Import Frap Pset1Sig.
+
+(* Authors: Peng Wang (wangpeng@csail.mit.edu), Adam Chlipala (adamc@csail.mit.edu) *)
+
+
+(** * MapReduce *)
+
+Lemma add_positive : forall n m,
+  n > 0
+  -> m > 0
+  -> n + m > 0.
+Proof.
+  linear_arithmetic.
+Qed.
+
+Theorem allPositive_ok : forall m x,
+  allPositive m
+  -> x > 0
+  -> interp_map m x > 0.
+Proof.
+  induct m; simplify; propositional.
+
+  apply add_positive.
+  apply IHm1.
+  trivial.
+  trivial.
+  apply IHm2.
+  trivial.
+  trivial.
+
+  apply IHm1.
+  trivial.
+  apply IHm2.
+  trivial.
+  trivial.
+Qed.
+
+Lemma fold_left_swap' : forall A (f : A -> A -> A),
+  (forall x y : A, f x y = f y x)
+  (* Operator is commutative. *)
+  -> (forall x y z : A, f (f x y) z = f x (f y z))
+  (* Operator is associative. *)
+  -> forall ls a b,
+      fold_left f ls (f a b) = f (fold_left f ls a) b.
+Proof.
+  induct ls; simplify; try equality.
+Qed.
+
+Lemma fold_left_swap : forall A (f : A -> A -> A),
+  (forall x y : A, f x y = f y x)
+  (* Operator is commutative. *)
+  -> (forall x y z : A, f (f x y) z = f x (f y z))
+  (* Operator is associative. *)
+  -> forall ls1 ls2 init,
+      fold_left f (ls1 ++ ls2) init = fold_left f (ls2 ++ ls1) init.
+Proof.
+  induct ls1; simplify.
+  {
+    rewrite app_nil_r.
+    equality.
+  }
+  {
+    rewrite IHls1.
+    rewrite fold_left_app.
+    rewrite fold_left_app.
+    simplify.
+    f_equal.
+    apply fold_left_swap'; trivial.
+  }
+Qed.
+
+Lemma reduce_swap : forall e ls1 ls2,
+  interp_reduce e (ls1 ++ ls2) = interp_reduce e (ls2 ++ ls1).
+Proof.
+  unfold interp_reduce; simplify.
+  cases e; apply fold_left_swap; simplify; linear_arithmetic.
+Qed.
+
+Lemma interp_swap : forall e ls1 ls2, interp_mr e (ls1 ++ ls2) = interp_mr e (ls2 ++ ls1).
+Proof.
+  induct e; simplify.
+  unfold interp_mr; simplify.
+  rewrite map_app.
+  rewrite map_app.
+  apply reduce_swap.
+Qed.
+
+Lemma fold_left_par' : forall A (f : A -> A -> A) (rzero : A),
+    (forall x y z : A, f (f x y) z = f x (f y z))
+    (* Operator is associative. *)
+    -> (forall x, f x rzero = x)
+    (* [rzero] is a right zero for operator. *)
+    -> forall ls init, fold_left f ls init = f init (fold_left f ls rzero).
+Proof.
+  induct ls; simplify; equality.
+Qed.
+
+Lemma fold_left_par : forall A (f : A -> A -> A) (rzero : A),
+    (forall x y z : A, f (f x y) z = f x (f y z))
+    (* Operator is associative. *)
+    -> (forall x, f x rzero = x)
+    (* [rzero] is a right zero for operator. *)
+    -> forall ls1 ls2 init,
+        fold_left f (ls1 ++ ls2) init = f (fold_left f ls1 init) (fold_left f ls2 rzero).
+Proof.
+  induct ls1; simplify; try equality.
+  apply fold_left_par'.
+  trivial.
+  trivial.
+Qed.
+
+Lemma mapReduce_partition_two : forall m r ls1 ls2,
+    interp_mr (m, r) (ls1 ++ ls2) = interp_reduce r [interp_mr (m, r) ls1; interp_mr (m, r) ls2].
+Proof.
+  unfold interp_mr; simplify.
+  cases r; simplify; rewrite map_app; apply fold_left_par; linear_arithmetic.
+Qed.
+
+Arguments app {_} _ _ .
+
+Lemma mapReduce_partition' : forall m r lsls init,
+    interp_mr (m, r) (fold_left app lsls init)
+    = interp_reduce r (interp_mr (m, r) init :: map (interp_mr (m, r)) lsls).
+Proof.
+  induct lsls; simplify.
+  {
+    unfold interp_reduce; simplify.
+    cases r; linear_arithmetic.
+  }
+  {
+    rewrite IHlsls.
+    rewrite mapReduce_partition_two.
+    cases r; simplify; linear_arithmetic.
+  }
+Qed.
+
+Lemma mapReduce_partition : forall m r lsls,
+    interp_mr (m, r) (fold_left app lsls []) = interp_reduce r (map (interp_mr (m, r)) lsls).
+Proof.
+  induct lsls; simplify; try equality.
+  apply mapReduce_partition'.
+Qed.
+
+
+(** * Constant propagation *)
+
+Theorem constPropArith_ok : forall v1 v2 e,
+  (forall x n, v1 $? x = Some n -> v2 $? x = Some n)
+  -> interp (constPropArith e v1) v2 = interp e v2.
+Proof.
+  induct e; simplify; propositional.
+
+  cases (v1 $? x); simplify; try equality.
+  rewrite (H x n); simplify; equality.
+
+  cases (constPropArith e1 v1); simplify; try equality.
+  cases (constPropArith e2 v1); simplify; equality.
+
+  cases (constPropArith e1 v1); simplify; try equality.
+  cases (constPropArith e2 v1); simplify; equality.
+
+  cases (constPropArith e1 v1); simplify; try equality.
+  cases (constPropArith e2 v1); simplify; equality.
+Qed.
+
+Theorem effectOf_ok : forall c v1 v2,
+  (forall x n, v1 $? x = Some n -> v2 $? x = Some n)
+  -> (forall x n, effectOf c v1 $? x = Some n
+                  -> exec c v2 $? x = Some n).
+Proof.
+  induct c; simplify; try equality.
+
+  apply H.
+  trivial.
+
+  cases (constPropArith e v1).
+  rewrite <- (constPropArith_ok v1).
+  cases (x ==v x0); simplify; try equality.
+  rewrite Heq.
+  simplify.
+  trivial.
+  apply H.
+  trivial.
+  trivial.
+
+  cases (x ==v x0); simplify; try equality.
+  apply H.
+  trivial.
+
+  cases (x ==v x0); simplify; try equality.
+  apply H.
+  trivial.
+
+  cases (x ==v x0); simplify; try equality.
+  apply H.
+  trivial.
+
+  cases (x ==v x0); simplify; try equality.
+  apply H.
+  trivial.
+
+  apply (IHc2 (effectOf c1 v1)).
+  apply IHc1.
+  trivial.
+  trivial.
+Qed.
+
+Theorem constProp_ok : forall c v1 v2,
+  (forall x n, v1 $? x = Some n -> v2 $? x = Some n)
+  -> exec (constProp c v1) v2 = exec c v2.
+Proof.
+  induct c; simplify; propositional.
+
+  rewrite constPropArith_ok.
+  trivial.
+  trivial.
+
+  rewrite IHc1.
+  rewrite IHc2.
+  trivial.
+  trivial.
+  apply effectOf_ok.
+  trivial.
+  trivial.
+
+  rewrite constPropArith_ok.
+  apply selfCompose_extensional.
+  simplify.
+  apply IHc.
+  simplify.
+  equality.
+  trivial.
+Qed.  
+
+Theorem constProp_ok0 : forall c v,
+  exec (constProp c $0) v = exec c v.
+Proof.
+  simplify.
+  apply constProp_ok.
+  simplify.
+  equality.
+Qed.
