pset2/Pset2Sol.v
@@ -1,0 +1,296 @@
+(** * 6.887 Formal Reasoning About Programs, Spring 2016 - Pset 2 *)
+
+Require Import Frap Pset2Sig.
+
+Set Implicit Arguments.
+
+
+(* Authors: Adam Chlipala (adamc@csail.mit.edu), Peng Wang (wangpeng@csail.mit.edu) *)
+
+Definition flag_for (pr : increment_program) : bool :=
+  match pr with
+    | SetFlag => false
+    | SetTurn => true
+    | ReadFlag => true
+    | ReadTurn => true
+    | Read => true
+    | Write _ => true
+    | UnsetFlag => true
+    | Done => false
+  end.
+
+Definition contribution_from (pr : increment_program) : nat :=
+  match pr with
+  | UnsetFlag => 1
+  | Done => 1
+  | _ => 0
+  end.
+
+Definition in_critical_section (pr : increment_program) : Prop :=
+  match pr with
+  | Read => True
+  | Write _ => True
+  | UnsetFlag => True
+  | _ => False
+  end.
+
+Definition instruction_ok (self other : increment_program) :=
+  match self with
+    | Write n => n = contribution_from other
+    | _ => True
+  end.
+
+Inductive increment2_invariant : threaded_state inc_state (increment_program * increment_program) -> Prop :=
+| Inc2Inv : forall tu pr1 pr2,
+  instruction_ok pr1 pr2
+  -> instruction_ok pr2 pr1
+  -> (in_critical_section pr1
+      -> (pr2 = SetFlag \/ pr2 = Done)
+         \/ (tu = false /\ (pr2 = ReadFlag \/ pr2 = ReadTurn))
+         \/ pr2 = SetTurn)
+  -> (in_critical_section pr2
+      -> (pr1 = SetFlag \/ pr1 = Done)
+         \/ (tu = true /\ (pr1 = ReadFlag \/ pr1 = ReadTurn))
+         \/ pr1 = SetTurn)
+  -> increment2_invariant {| Shared :=
+                               {| Flag1 := flag_for pr1; Flag2 := flag_for pr2; Turn := tu;
+                                  Global := contribution_from pr1 + contribution_from pr2 |};
+                             Private := (pr1, pr2) |}.
+
+Lemma Inc2Inv' : forall sh tu pr1 pr2,
+  sh = {| Flag1 := flag_for pr1; Flag2 := flag_for pr2; Turn := tu;
+          Global := contribution_from pr1 + contribution_from pr2 |}
+  -> instruction_ok pr1 pr2
+  -> instruction_ok pr2 pr1
+  -> (in_critical_section pr1
+      -> (pr2 = SetFlag \/ pr2 = Done)
+         \/ (tu = false /\ (pr2 = ReadFlag \/ pr2 = ReadTurn))
+         \/ pr2 = SetTurn)
+  -> (in_critical_section pr2
+      -> (pr1 = SetFlag \/ pr1 = Done)
+         \/ (tu = true /\ (pr1 = ReadFlag \/ pr1 = ReadTurn))
+         \/ pr1 = SetTurn)
+  -> increment2_invariant {| Shared := sh; Private := (pr1, pr2) |}.
+Proof.
+  simplify.
+  rewrite H.
+  apply Inc2Inv; assumption.
+Qed.
+
+Theorem increment2_ok :
+  invariantFor increment2_sys increment2_correct.
+Proof.
+  apply invariant_weaken with (invariant1 := increment2_invariant).
+
+  apply invariant_induction; simplify.
+
+  invert H.
+  invert H0.
+  invert H1.
+  eapply Inc2Inv'.
+  equality.
+  simplify.
+  trivial.
+  simplify.
+  trivial.
+  simplify.
+  propositional.
+  simplify.
+  propositional.
+
+  invert H.
+  invert H0.
+
+  invert H8; simplify.
+
+  eapply Inc2Inv'.
+  simplify.
+  equality.
+  simplify.
+  trivial.
+  cases pr2; simplify; trivial.
+  simplify.
+  propositional.
+  propositional.
+
+  eapply Inc2Inv'.
+  simplify.
+  equality.
+  simplify.
+  trivial.
+  cases pr2; simplify; trivial.
+  simplify.
+  propositional.
+  propositional.
+
+  eapply Inc2Inv'.
+  simplify.
+  equality.
+  simplify.
+  trivial.
+  cases pr2; simplify; trivial.
+  simplify.
+  propositional.
+  equality.
+
+  eapply Inc2Inv'.
+  simplify.
+  equality.
+  simplify.
+  trivial.
+  cases pr2; simplify; trivial.
+  simplify.
+  cases pr2; simplify; equality.
+  cases pr2; simplify; equality.
+
+  eapply Inc2Inv'.
+  simplify.
+  equality.
+  simplify.
+  trivial.
+  cases pr2; simplify; trivial.
+  simplify.
+  cases pr2; simplify; equality.
+  cases pr2; simplify; equality.
+
+  eapply Inc2Inv'.
+  simplify.
+  equality.
+  simplify.
+  trivial.
+  cases pr2; simplify; trivial.
+  simplify.
+  cases pr2; simplify; equality.
+  cases pr2; simplify; equality.
+
+  eapply Inc2Inv'.
+  simplify.
+  equality.
+  simplify.
+  trivial.
+  cases pr2; simplify; trivial.
+  simplify.
+  cases pr2; simplify; equality.
+  cases pr2; simplify; equality.
+
+  eapply Inc2Inv'.
+  simplify.
+  rewrite H1.
+  equality.
+  simplify.
+  trivial.
+  cases pr2; simplify; trivial.
+  equality.
+  simplify.
+  cases pr2; simplify; equality.
+  cases pr2; simplify; equality.
+
+  eapply Inc2Inv'.
+  simplify.
+  equality.
+  simplify.
+  trivial.
+  cases pr2; simplify; trivial.
+  cases pr2; simplify; equality.
+  cases pr2; simplify; equality.
+
+  invert H8; simplify.
+
+  eapply Inc2Inv'.
+  simplify.
+  equality.
+  cases pr1; simplify; trivial.
+  simplify.
+  trivial.
+  simplify.
+  propositional.
+  propositional.
+
+  eapply Inc2Inv'.
+  simplify.
+  equality.
+  cases pr1; simplify; trivial.
+  simplify.
+  trivial.
+  simplify.
+  propositional.
+  cases pr1; simplify; propositional.
+
+  eapply Inc2Inv'.
+  simplify.
+  equality.
+  cases pr1; simplify; trivial.
+  simplify.
+  trivial.
+  simplify.
+  cases pr1; simplify; equality.
+  equality.
+
+  eapply Inc2Inv'.
+  simplify.
+  equality.
+  cases pr1; simplify; trivial.
+  simplify.
+  trivial.
+  simplify.
+  cases pr1; simplify; equality.
+  cases pr1; simplify; equality.
+
+  eapply Inc2Inv'.
+  simplify.
+  equality.
+  cases pr1; simplify; trivial.
+  simplify.
+  trivial.
+  simplify.
+  cases pr1; simplify; equality.
+  cases pr1; simplify; equality.
+
+  eapply Inc2Inv'.
+  simplify.
+  equality.
+  cases pr1; simplify; trivial.
+  simplify.
+  trivial.
+  simplify.
+  cases pr1; simplify; equality.
+  cases pr1; simplify; equality.
+
+  eapply Inc2Inv'.
+  simplify.
+  equality.
+  cases pr1; simplify; trivial.
+  simplify.
+  trivial.
+  simplify.
+  cases pr1; simplify; equality.
+  cases pr1; simplify; equality.
+  cases pr1; simplify; equality.
+
+  eapply Inc2Inv'.
+  simplify.
+  f_equal.
+  linear_arithmetic.
+  cases pr1; simplify; trivial.
+  equality.
+  simplify.
+  trivial.
+  simplify.
+  cases pr1; simplify; equality.
+  cases pr1; simplify; equality.
+
+  eapply Inc2Inv'.
+  simplify.
+  equality.
+  cases pr1; simplify; trivial.
+  simplify.
+  trivial.
+  cases pr1; simplify; equality.
+  cases pr1; simplify; equality.
+  
+  invert 1.
+  unfold increment2_correct; simplify.
+  invert H.
+  simplify.
+  equality.
+Qed.
