pset1/Pset1-2.v
@@ -1,0 +1,12 @@
+1 subgoals, subgoal 1 (ID 1209)
+  
+  m : map_
+  r : reduce
+  a : list nat
+  lsls : list (list nat)
+  IHlsls : interp_mr (m, r) (fold_left app lsls []) =
+           interp_reduce r (map (interp_mr (m, r)) lsls)
+  ============================
+   interp_mr (m, r) (fold_left app lsls a) =
+   interp_reduce r (interp_mr (m, r) a :: map (interp_mr (m, r)) lsls)
+
